ems/SimSTS2.v
@@ -47,46 +47,46 @@ Proof.
   }
 Qed.
 
-Variant indC (of_state: L.(state) -> Tr.t -> Prop): L.(state) -> Tr.t -> Prop :=
-| indC_final
+Variant of_state_indC (of_state: L.(state) -> Tr.t -> Prop): L.(state) -> Tr.t -> Prop :=
+| of_state_indC_final
     st0 retv
     (FINAL: L.(state_sort) st0 = final retv)
   :
-    indC of_state st0 (Tr.done retv)
-| indC_spin
+    of_state_indC of_state st0 (Tr.done retv)
+| of_state_indC_spin
     st0
     (SPIN: Beh.state_spin L st0)
   :
-    indC of_state st0 (Tr.spin)
-| indC_nb
+    of_state_indC of_state st0 (Tr.spin)
+| of_state_indC_nb
     st0
   :
-    indC of_state st0 (Tr.nb)
-| indC_vis
+    of_state_indC of_state st0 (Tr.nb)
+| of_state_indC_vis
     st0 st1 ev evs
     (SRT: L.(state_sort) st0 = vis)
     (STEP: _.(step) st0 (Some ev) st1)
     (TL: of_state st1 evs)
   :
-    indC of_state st0 (Tr.cons ev evs)
-| indC_demonic
+    of_state_indC of_state st0 (Tr.cons ev evs)
+| of_state_indC_demonic
     st0
     evs
     (SRT: L.(state_sort) st0 = demonic)
     (STEP: Beh.union L st0 (fun e st1 => (<<HD: e = None>>) /\ (<<TL: of_state st1 evs>>)))
   :
-    indC of_state st0 evs
-| indC_angelic
+    of_state_indC of_state st0 evs
+| of_state_indC_angelic
     st0
     evs
     (SRT: L.(state_sort) st0 = angelic)
     (STEP: Beh.inter L st0 (fun e st1 => (<<HD: e = None>>) /\ (<<TL: of_state st1 evs>>)))
   :
-    indC of_state st0 evs
+    of_state_indC of_state st0 evs
 .
 
-Lemma indC_mon:
-  monotone2 indC.
+Lemma of_state_indC_mon:
+  monotone2 of_state_indC.
 Proof.
   ii. inv IN; eauto.
   - econs 1; eauto.
@@ -96,10 +96,10 @@ Proof.
   - econs 5; eauto. unfold Beh.union in *. des. esplits; eauto.
   - econs 6; eauto. ii. exploit STEP; eauto. i. des. splits; auto.
 Qed.
-Hint Resolve indC_mon: paco.
+Hint Resolve of_state_indC_mon: paco.
 
-Lemma indC_spec:
-  indC <3= gupaco2 (Beh._of_state L) (cpn2 (Beh._of_state L)).
+Lemma of_state_indC_spec:
+  of_state_indC <3= gupaco2 (Beh._of_state L) (cpn2 (Beh._of_state L)).
 Proof.
   eapply wrespect2_uclo; eauto with paco.
   econs; eauto with paco.
@@ -171,7 +171,7 @@ Section SIM.
       (SIM: exists st_src1
                    (STEP: _.(step) st_src0 None st_src1)
         ,
-          exists i_src1, <<SIM: _sim sim i_src1 i_tgt0 st_src1 st_tgt0>>)
+          <<SIM: _sim sim true i_tgt0 st_src1 st_tgt0>>)
     :
       _sim sim i_src0 i_tgt0 st_src0 st_tgt0
   | sim_demonic_tgt
@@ -180,7 +180,7 @@ Section SIM.
       (SIM: forall st_tgt1
                    (STEP: _.(step) st_tgt0 None st_tgt1)
         ,
-          exists i_tgt1, <<SIM: _sim sim i_src0 i_tgt1 st_src0 st_tgt1>>)
+          <<SIM: _sim sim i_src0 true st_src0 st_tgt1>>)
     :
       _sim sim i_src0 i_tgt0 st_src0 st_tgt0
   | sim_progress
@@ -204,7 +204,7 @@ Section SIM.
             (SIM: exists st_src1
                          (STEP: _.(step) st_src0 None st_src1)
               ,
-                exists i_src1, <<SIM: _sim sim i_src1 i_tgt0 st_src1 st_tgt0>> /\ <<IH: P i_src1 i_tgt0 st_src1 st_tgt0>>),
+                <<SIM: _sim sim true i_tgt0 st_src1 st_tgt0>> /\ <<IH: P true i_tgt0 st_src1 st_tgt0>>),
             P i_src0 i_tgt0 st_src0 st_tgt0)
         (DMTGT: forall
             i_src0 i_tgt0 st_src0 st_tgt0
@@ -212,7 +212,7 @@ Section SIM.
             (SIM: forall st_tgt1
                          (STEP: _.(step) st_tgt0 None st_tgt1)
               ,
-                exists i_tgt1, <<SIM: _sim sim i_src0 i_tgt1 st_src0 st_tgt1>> /\ <<IH: P i_src0 i_tgt1 st_src0 st_tgt1>>),
+                <<SIM: _sim sim i_src0 true st_src0 st_tgt1>> /\ <<IH: P i_src0 true st_src0 st_tgt1>>),
             P i_src0 i_tgt0 st_src0 st_tgt0)
         (PROGRESS:
            forall
@@ -231,7 +231,7 @@ Section SIM.
     { eapply DMSRC; eauto.
       des. esplits; eauto. }
     { eapply DMTGT; eauto. i.
-      hexploit SIM0; eauto. i. des. esplits; eauto. }
+      hexploit SIM0; eauto. }
     { eapply PROGRESS; eauto. }
   Qed.
 
@@ -249,6 +249,7 @@ Section SIM.
   Hint Constructors _sim.
   Hint Unfold sim.
   Hint Resolve sim_mon: paco.
+  Hint Resolve cpn4_wcompat: paco.
 
   Lemma sim_ind (P: bool -> bool -> L0.(state) -> L1.(state) -> Prop)
         (FIN: forall
@@ -263,7 +264,7 @@ Section SIM.
             (SIM: exists st_src1
                          (STEP: _.(step) st_src0 None st_src1)
               ,
-                exists i_src1, <<SIM: sim i_src1 i_tgt0 st_src1 st_tgt0>> /\ <<IH: P i_src1 i_tgt0 st_src1 st_tgt0>>),
+                <<SIM: sim true i_tgt0 st_src1 st_tgt0>> /\ <<IH: P true i_tgt0 st_src1 st_tgt0>>),
             P i_src0 i_tgt0 st_src0 st_tgt0)
         (DMTGT: forall
             i_src0 i_tgt0 st_src0 st_tgt0
@@ -271,7 +272,7 @@ Section SIM.
             (SIM: forall st_tgt1
                          (STEP: _.(step) st_tgt0 None st_tgt1)
               ,
-                exists i_tgt1, <<SIM: sim i_src0 i_tgt1 st_src0 st_tgt1>> /\ <<IH: P i_src0 i_tgt1 st_src0 st_tgt1>>),
+                <<SIM: sim i_src0 true st_src0 st_tgt1>> /\ <<IH: P i_src0 true st_src0 st_tgt1>>),
             P i_src0 i_tgt0 st_src0 st_tgt0)
         (PROGRESS:
            forall
@@ -293,6 +294,102 @@ Section SIM.
       pfold. eapply sim_mon; eauto.
     }
     { punfold SIM. eapply sim_mon; eauto. i. pclearbot. auto. }
+  Qed.
+
+  Variant sim_indC (sim: bool -> bool -> L0.(state) -> L1.(state) -> Prop)
+          (i_src0: bool) (i_tgt0: bool) (st_src0: L0.(state)) (st_tgt0: L1.(state)): Prop :=
+  | sim_indC_fin
+      retv
+      (SRT: _.(state_sort) st_src0 = final retv)
+      (SRT: _.(state_sort) st_tgt0 = final retv)
+    :
+      sim_indC sim i_src0 i_tgt0 st_src0 st_tgt0
+  | sim_indC_demonic_src
+      (SRT: _.(state_sort) st_src0 = demonic)
+      (SIM: exists st_src1
+                   (STEP: _.(step) st_src0 None st_src1)
+        ,
+          <<SIM: sim true i_tgt0 st_src1 st_tgt0>>)
+    :
+      sim_indC sim i_src0 i_tgt0 st_src0 st_tgt0
+  | sim_indC_demonic_tgt
+      (SRT: _.(state_sort) st_tgt0 = demonic)
+      (SIM: forall st_tgt1
+                   (STEP: _.(step) st_tgt0 None st_tgt1)
+        ,
+          <<SIM: sim i_src0 true st_src0 st_tgt1>>)
+    :
+      sim_indC sim i_src0 i_tgt0 st_src0 st_tgt0
+  | sim_indC_progress
+      (SIM: sim false false st_src0 st_tgt0)
+      (SRC: i_src0 = true)
+      (TGT: i_tgt0 = true)
+    :
+      sim_indC sim i_src0 i_tgt0 st_src0 st_tgt0
+  .
+
+  Lemma sim_indC_mon: monotone4 sim_indC.
+  Proof.
+    ii. inv IN; eauto.
+    { econs 1; eauto. }
+    { econs 2; eauto. des. esplits; eauto. }
+    { econs 3; eauto. i. hexploit SIM; eauto. }
+    { econs 4; eauto. }
+  Qed.
+  Hint Resolve sim_indC_mon: paco.
+
+  Lemma sim_indC_spec:
+    sim_indC <5= gupaco4 _sim (cpn4 _sim).
+  Proof.
+    eapply wrespect4_uclo; eauto with paco.
+    econs; eauto with paco. i. inv PR.
+    { econs 1; eauto. }
+    { econs 2; eauto. des. esplits; eauto.
+      eapply sim_mon; eauto. i. eapply rclo4_base. auto.
+    }
+    { econs 3; eauto. i. hexploit SIM; eauto. i.
+      eapply sim_mon; eauto. i. eapply rclo4_base. auto.
+    }
+    { econs 4; eauto. eapply rclo4_base. auto. }
+  Qed.
+
+  Variant sim_flagC (sim: bool -> bool -> L0.(state) -> L1.(state) -> Prop)
+          (i_src1: bool) (i_tgt1: bool) (st_src: L0.(state)) (st_tgt: L1.(state)): Prop :=
+  | sim_flagC_intro
+      i_src0 i_tgt0
+      (SIM: sim i_src0 i_tgt0 st_src st_tgt)
+      (SRC: i_src0 = true -> i_src1 = true)
+      (TGT: i_tgt0 = true -> i_tgt1 = true)
+  .
+
+  Lemma sim_flagC_mon: monotone4 sim_flagC.
+  Proof.
+    ii. inv IN; eauto. econs; eauto.
+  Qed.
+  Hint Resolve sim_flagC_mon: paco.
+
+  Lemma sim_flagC_spec:
+    sim_flagC <5= gupaco4 _sim (cpn4 _sim).
+  Proof.
+    eapply wrespect4_uclo; eauto with paco.
+    econs; eauto with paco. i. inv PR.
+    eapply GF in SIM.
+    revert x0 x1 SRC TGT. induction SIM using _sim_ind2; i; clarify.
+    { econs 1; eauto. }
+    { econs 2; eauto. des. esplits; eauto. }
+    { econs 3; eauto. i. exploit SIM; eauto. i. des. eauto. }
+    { econs 4; eauto. eapply rclo4_base. auto. }
+  Qed.
+
+  Lemma sim_flag_mon:
+    forall f_src0 f_tgt0 f_src1 f_tgt1 st_src st_tgt
+           (SIM: sim f_src0 f_tgt0 st_src st_tgt)
+           (SRC: f_src0 = true -> f_src1 = true)
+           (TGT: f_tgt0 = true -> f_tgt1 = true),
+      sim f_src1 f_tgt1 st_src st_tgt.
+  Proof.
+    ginit. i. guclo sim_flagC_spec. econs; eauto.
+    gfinal. right. eauto.
   Qed.
 
   Record simulation: Prop := mk_simulation {
@@ -349,6 +446,57 @@ Section SIM.
     { i. eapply cpn2_wcompat; eauto. eapply Beh.of_state_mon. }
     revert i_tgt0 i_src0 st_src0 st_tgt0 SIM. gcofix CIH.
     i. rename x2 into tr.
+    cut (sim true i_tgt0 st_src0 st_tgt0).
+    2:{ eapply sim_flag_mon; eauto. }
+    clear i_src0 SIM. intros SIM.
+    match goal with
+    | |- ?goal => cut (goal \/ true = false)
+    end.
+    { i. des; ss. }
+    revert SIM. generalize true. intros i_src0 SIM.
+    revert i_src0 i_tgt0 st_src0 SIM.
+    induction PR using of_state_ind2; ii; ss; rename st0 into st_tgt0.
+    - (** done **)
+      revert retv H.
+      induction SIM using sim_ind; i; clarify.
+      + rewrite SRT0 in *. clarify. left. gstep. econs; eauto.
+      + des. left. exploit IH; eauto. i; des; ss.
+        guclo of_state_indC_spec. econs 5; eauto. red. esplits; eauto.
+      + rewrite SRT in *. clarify.
+      + revert SIM.
+
+        admitt.
+    - (** spin **)
+      left. exploit adequacy_spin; eauto. i.
+      gstep. econs. et.
+    - (** nb **)
+      left. gstep. econs; eauto.
+    - (** cons **)
+      revert ev SRT STEP.
+      induction SIM using sim_ind; i; try rewrite SRT0 in *; clarify.
+      * des. exploit IH; eauto. i. des; ss. left.
+        guclo of_state_indC_spec. econs 5; eauto. red. esplits; eauto.
+      * auto.
+
+      cut (sim false i_tgt0 st_src0 st_tgt0).
+      2:{ admitt. }
+      clear SIM i_src0. intros SIM.
+      match goal with
+      | |- ?goal => cut (goal \/ true = false)
+      end.
+      { i. des; ss. }
+
+  Lemma adequacy_aux
+        i_src0 i_tgt0 st_src0 st_tgt0
+        (SIM: sim i_src0 i_tgt0 st_src0 st_tgt0)
+    :
+      <<IMPR: Beh.improves (Beh.of_state L0 st_src0) (Beh.of_state L1 st_tgt0)>>
+  .
+  Proof.
+    ginit.
+    { i. eapply cpn2_wcompat; eauto. eapply Beh.of_state_mon. }
+    revert i_tgt0 i_src0 st_src0 st_tgt0 SIM. gcofix CIH.
+    i. rename x2 into tr.
     punfold PR. revert i_src0 i_tgt0 st_src0 SIM.
     induction PR using Beh.of_state_ind; ii; ss; rename st0 into st_tgt0.
     - (** done **)
@@ -364,20 +512,71 @@ Section SIM.
     - (** nb **)
       gstep. econs; eauto.
     - (** cons **)
+      cut (sim false i_tgt0 st_src0 st_tgt0).
+      2:{ admitt. }
+      clear SIM i_src0. intros SIM.
+      match goal with
+      | |- ?goal => cut (goal \/ true = false)
+      end.
+      { i. des; ss. }
+
+
       pc TL. induction SIM using sim_ind; i; try rewrite SRT in *; clarify.
       + (** d_ **)
         des. guclo indC_spec. econs 5; eauto. red. esplits; eauto.
       + (** progress **)
-        remember false in SIM at 1.
-        remember false in SIM at 1.
-        clear Heqb0. revert Heqb.
+        match goal with
+        | |- ?goal => cut (goal \/ true = false)
+        end.
+        { i. des; ss. }
+        revert SIM. generalize false at 2 3.
+        generalize false at 1. intros f_src f_tgt SIM.
         revert ev SRT STEP.
         induction SIM using sim_ind; i; try rewrite SRT0 in *; clarify.
-        * des. guclo indC_spec. econs 5; eauto. red. esplits; eauto.
-
-          exploit IH; eauto. i.
+        * des. exploit IH; eauto. i. des; auto. left.
           guclo indC_spec. econs 5; eauto. red. esplits; eauto.
-        *
+        * auto.
+
+
+    - (** cons **)
+      pc TL. induction SIM using sim_ind; i; try rewrite SRT in *; clarify.
+      + (** d_ **)
+        des. guclo indC_spec. econs 5; eauto. red. esplits; eauto.
+      + (** progress **)
+        match goal with
+        | |- ?goal => cut (goal \/ true = false)
+        end.
+        { i. des; ss. }
+        revert SIM. generalize false at 2 3.
+        generalize false at 1. intros f_src f_tgt SIM.
+        revert ev SRT STEP.
+        induction SIM using sim_ind; i; try rewrite SRT0 in *; clarify.
+        * des. exploit IH; eauto. i. des; auto. left.
+          guclo indC_spec. econs 5; eauto. red. esplits; eauto.
+        * auto.
+    - (** demonic **)
+      red in STEP. des. clarify.
+      induction SIM using sim_ind; i; try rewrite SRT in *; clarify.
+      + des. hexploit IH0; eauto. i.
+        guclo indC_spec. econs 5; eauto. red. esplits; eauto.
+      + hexploit SIM; eauto. i. des. eapply IH; eauto.
+      +
+
+        des. hexploit IH; eauto.
+
+
+      revert i_src0 st_src0 SIM.
+      induction (WFTGT i_tgt0).
+      clear H. rename x into i_tgt0. rename H0 into IHTGT. i.
+      rr in STEP. des. clarify. rename st1 into st_tgt1.
+      punfold SIM. inv SIM; try rewrite SRT in *; ss.
+      + des. pc SIM.
+        guclo Beh.dstep_clo_spec. econs; et.
+      + exploit SIM0; et. i. des. pc SIM.
+        eapply IH; et.
+      + guclo Beh.astep_clo_spec. econs; et. ii.
+        exploit SIM0; et. i. des. pc SIM. et.
+    -
 
 
           rewrite SRT0 in *. clarify.
